theories/Util.v
@@ -3,7 +3,9 @@
  *
  * SPDX-License-Identifier:AGPL-3.0-or-later
  *)
+Require Import Coq.Classes.DecidableClass.
 Require Import Coq.Lists.List.
+Require Import Coq.Strings.String.
 
 (* note(gmm): this file should be eliminated in favor of definitions defined elsewhere, e.g. in ExtLib *)
 
@@ -21,3 +23,98 @@ Section find_in_list.
       end
     end.
 End find_in_list.
+
+Global Instance Decidable_eq_string (a b : string) : Decidable (a = b) :=
+  {| Decidable_witness := String.eqb a b
+   ; Decidable_spec := @String.eqb_eq a b |}.
+
+Section dec_list.
+  Context {T : Type} {dec : forall a b : T, Decidable (a = b)}.
+
+  Fixpoint dec_list (a b : list T) : bool :=
+    match a , b with
+    | nil , nil => true
+    | x :: xs , y :: ys => decide (x = y) && dec_list xs ys
+    | _ , _ => false
+    end.
+
+  Lemma dec_list_ok:
+    forall a b : list T, dec_list a b = true <-> a = b.
+  Proof.
+    induction a; destruct b; simpl; intros; try solve [ tauto | split; congruence ].
+    split.
+    - intros. eapply Bool.andb_true_iff in H. destruct H.
+      eapply Decidable_sound in H.
+      eapply IHa in H0. f_equal; assumption.
+    - inversion 1; subst.
+      eapply Bool.andb_true_iff.
+      split.
+      eapply Decidable_complete. auto.
+      eapply IHa. reflexivity.
+  Qed.
+
+  Global Instance Decidable_eq_list (a b : list T) : Decidable (a = b) :=
+  {| Decidable_witness := dec_list a b
+   ; Decidable_spec := dec_list_ok a b |}.
+
+  Definition dec_option (a b : option T) : bool :=
+    match a , b with
+    | None , None => true
+    | Some a , Some b => decide (a = b)
+    | _ , _ => false
+    end.
+
+  Lemma dec_option_ok : forall a b, dec_option a b = true <-> a = b.
+  Proof.
+    destruct a; destruct b; simpl; try solve [ tauto | split; congruence ].
+    generalize (dec t t0).
+    destruct d.
+    simpl. etransitivity. eassumption.
+    split; congruence.
+  Qed.
+
+  Global Instance Decidable_eq_option (a b : option T) : Decidable (a = b) :=
+  {| Decidable_witness := dec_option a b
+   ; Decidable_spec := dec_option_ok a b |}.
+
+End dec_list.
+
+Section dec_sum.
+  Context {T U : Type}
+          {decT : forall a b : T, Decidable (a = b)}
+          {decU : forall a b : U, Decidable (a = b)}.
+
+  Definition dec_sum (a b : T + U) : bool :=
+    match a , b with
+    | inl a , inl b => decide (a = b)
+    | inr a , inr b => decide (a = b)
+    | _ , _ => false
+    end.
+
+  Lemma dec_sum_ok : forall a b, dec_sum a b = true <-> a = b.
+  Proof.
+    destruct a; destruct b; simpl; try solve [ split; congruence ].
+    all: etransitivity; [ eapply Decidable_spec | split; congruence ].
+  Qed.
+
+  Global Instance Decidable_eq_sum (a b : T + U) : Decidable (a = b) :=
+  {| Decidable_witness := dec_sum a b
+   ; Decidable_spec := dec_sum_ok a b |}.
+
+
+  Definition dec_prod (a b : T * U) : bool :=
+    decide (fst a = fst b) && decide (snd a = snd b).
+
+  Lemma dec_prod_ok : forall a b, dec_prod a b = true <-> a = b.
+  Proof.
+    destruct a; destruct b; unfold dec_prod; simpl; try solve [ split; congruence ].
+    etransitivity. eapply Bool.andb_true_iff.
+    do 2 rewrite Decidable_spec.
+    split; firstorder; congruence.
+  Qed.
+
+  Global Instance Decidable_eq_prod (a b : T * U) : Decidable (a = b) :=
+  {| Decidable_witness := dec_prod a b
+   ; Decidable_spec := dec_prod_ok a b |}.
+
+End dec_sum.
