tests/demo/A_o.v
@@ -14,36 +14,15 @@ From Demo Require
      A_cpp A_cpp_spec A_cpp_proof.
 Import A_hpp_spec.
 
-(* todo(gmm): I'm a bit confused about the appropriate specification of linking
- *)
-Lemma wand_apply : forall A B F F' : mpred,
-    F |-- A ** F' ->
-    (A -* B) ** F |-- B ** F'.
-Proof.
-  intros.
-  rewrite H.
-  work.
-  rewrite sepSPC.
-  eapply sepSPAdj.
-  reflexivity.
-Qed.
-
 Theorem A_o_sound (resolve : _)
-: |-- denoteModule (module_link A_hpp.module A_cpp.module) -*
-      (Forall ti, cglob (resolve:=resolve) A__foo ti A__foo_spec) **
-      (Forall ti, cglob (resolve:=resolve) A__bar ti A__bar_spec).
+: denoteModule A_cpp.module
+  |-- (ti_cglob (resolve:=resolve) A__foo A__foo_spec) **
+      (ti_cglob (resolve:=resolve) A__bar A__bar_spec).
 Proof.
-  eapply spec_lob.
-  eapply wandSPAdj.
-  rewrite denote_module_dup at 2.
-  rewrite denoteModule_link.
-  rewrite (A_cpp_proof.A_cpp_sound resolve) at 2.
-  rewrite (A_hpp_proof.A_hpp_sound resolve) at 2.
-  unfold A_hpp_spec, A_cpp_spec.A_cpp_spec.
-  do 2 Discharge.perm_right ltac:(idtac; Discharge.perm_left ltac:(eapply wand_apply)).
-  rewrite illater_wandSP.
-  rewrite <- illater_sepSP.
-  Discharge.perm_right ltac:(idtac; Discharge.perm_left ltac:(eapply wand_apply)).
-  rewrite <- spec_later_weaken.
-  Discharge.discharge fail idtac fail ltac:(Discharge.canceler fail eauto) eauto.
+  use_module (A_hpp_proof.A_hpp_sound resolve).
+  use_module (A_cpp_proof.A_cpp_sound resolve).
+  rewrite denoteModule_weaken.
+  unfold A_cpp_spec.A_cpp_spec.
+  unfold A_hpp_spec.A_hpp_spec.
+  module_cancel.
 Qed.
